app/Solver.v
@@ -1,0 +1,109 @@
+From HTTP Require Import
+     Tester.
+From App Require Export
+     Observe.
+
+Definition solver_state := list (var * option N).
+
+Definition unifyN (nx : exp N) (n : N) (s : solver_state)
+  : option solver_state :=
+  match nx with
+  | Exp__Var x =>
+    if get x s is Some (Some n0)
+    then if n0 =? n then Some s else None
+    else Some $ update x (Some n) s
+  | Exp__Const n0 => if n0 =? n then Some s else None
+  | Exp__Nth _ _  => None
+  end.
+
+Definition unifyOrder (s : solver_state) (ox : orderT exp) (o : orderT id)
+  : option solver_state :=
+  let '((oidx, (bix, bax, six, sax)), (oid, (bi, ba, si, sa))) := (ox, o) in
+  if (bax, sax) = (ba, sa)?
+  then unifyN oidx oid s >>= unifyN bix bi >>= unifyN six si
+  else None.
+
+Definition unifyAccount (s : solver_state) (ax : accountT exp) (a : accountT id)
+  : option solver_state :=
+  let '((aidx, vx), (aid, v)) := (ax, a) in
+  if vx = v? then unifyN aidx aid s else None.
+
+Definition unifyList {A : (Type -> Type) -> Type}
+           (unifier : solver_state -> A exp -> A id -> option solver_state)
+           (lx : list (A exp)) (l : list (A id)) (s : solver_state)
+  : option solver_state :=
+  if length lx =? length l
+  then fold_left (fun os ab => os >>= (fun s => uncurry (unifier s) ab))
+                 (zip lx l) (pure s)
+  else None.
+
+Definition get_value (s : solver_state) (x : exp N) : option N :=
+  match x with
+  | Exp__Var   x => join $ get x s
+  | Exp__Const n => Some n
+  | Exp__Nth _ _ => None
+  end.
+
+Fixpoint find_nth {A} (f : A -> bool) (l : list A) : nat :=
+  match l with
+  | [] => O
+  | a :: l' => if f a then O else S (find_nth f l')
+  end.
+
+Definition eval_nth (n : N) (l : list (exp N)) (s : solver_state) : nat :=
+  let l' : list (option N) := map (get_value s) l in
+  find_nth (fun on => on = Some n?) l'.
+
+Instance Serialize__idVar : Serialize (id var) :=
+  fun (a : var) => to_sexp a.
+
+Instance Serialize__IdResponse : Serialize (swap_response id) :=
+  Serialize__Response.
+
+Definition instantiate_unify {E A} `{failureE -< E} (e : unifyE swap_response A)
+  : Monads.stateT solver_state (itree E) A :=
+  fun s : solver_state =>
+    match e with
+    | Unify__Fresh =>
+      let x : var := fresh_var s in
+      ret (put x None s, Exp__Var x)
+    | Unify__Eval v =>
+      if v is Exp__Nth x l
+      then if get_value s x is Some n
+           then ret (s, eval_nth n l s)
+           else ret (s, length l)
+      else throw "Should not happen"
+    | Unify__Match rx r =>
+      let mismatch := throw $ "Expect " ++ to_string rx
+                            ++ " but observed " ++ to_string r in
+      let handle os' := if os' is Some s' then ret (s', tt) else mismatch in
+      match rx, r with
+      | Response__InsufficientFund, Response__InsufficientFund
+      | Response__NotFound        , Response__NotFound => ret (s, tt)
+      | Response__ListAccount lx  , Response__ListAccount l =>
+        handle $ unifyList (A:=accountT) unifyAccount lx l s
+      | Response__ListOrders  lx  , Response__ListOrders  l =>
+        handle $ unifyList (A:=orderT) unifyOrder lx l s
+      | Response__ListAccount [], Response__ListOrders  []
+      | Response__ListOrders  [], Response__ListAccount [] => ret (s, tt)
+      | Response__Account ax, Response__Account a => handle $ unifyAccount s ax a
+      | Response__Order   ox, Response__Order   o => handle $ unifyOrder   s ox o
+      | _, _ => mismatch
+      end
+    end.
+
+Definition solver' {E F} `{failureE -< E} `{F -< E}
+           (m : itree (unifyE swap_response +' F) void)
+  : Monads.stateT solver_state (itree E) void :=
+  interp
+    (fun _ e =>
+       match e with
+       | (ue|) => instantiate_unify ue
+       | (|ee)  => liftState (F:=itree _) (trigger ee)
+       end) m.
+
+Definition solver {E F} `{failureE -< E} `{F -< E}
+           (m : itree (unifyE swap_response +' F) void) : itree E void :=
+  snd <$> solver' m [].
+
+Definition solve_swap := solver ∘ observe_swap.
